Versión antes de añadir predicados opacos

Verification/VerificationCDPC.dfy
@@ -14,6 +14,7 @@ method verifyCDPC(f:Map_Map_T<int, bool, bool>, g:Map_Map_T<int, bool, int>, P:S
   requires forall c:candidate | c in f.Keys() :: (P.Model() <= c.Keys)
   requires 0.0 <= a <= b <= 1.0
   requires 0.0 <= x <= y <= 1.0
+  
   ensures r == certificateCDPC(f.Model(), g.Model(), P.Model(), a, b, x, y, iv.Model())
 {
   counter := counter_in;
@@ -33,18 +34,31 @@ method verifyCDPC(f:Map_Map_T<int, bool, bool>, g:Map_Map_T<int, bool, int>, P:S
     var question:int; question, counter := iv.Key(counter);
     var f':Map_Map_T<int, bool, bool>; f', counter := f.Copy(counter);
     var f'Empty:bool; f'Empty, counter := f'.Empty(counter);
-    var ok:bool := true;
+    var cands_have_question:bool := true;
+    var exists_answer_true:bool := false;
+    var exists_answer_false:bool := false;
     
-    while (!f'Empty)
+    while (!f'Empty && cands_have_question)
       decreases f'.Cardinality()
       invariant in_universe_Map_Map_T(f', f)
-      invariant ok == (forall cand:candidate | cand in (f.Keys() - f'.Keys()) :: question in cand.Keys)
+      invariant cands_have_question == (forall cand:candidate | cand in (f.Keys() - f'.Keys()) :: question in cand.Keys)
+      invariant cands_have_question ==> (exists_answer_true == (exists cand:candidate | cand in (f.Keys() - f'.Keys()) :: cand[question] == true))
+      invariant cands_have_question ==> (exists_answer_false == (exists cand:candidate | cand in (f.Keys() - f'.Keys()) :: cand[question] == false))
       invariant f'Empty == (f'.Cardinality() == 0)
     {
-      f', f'Empty, ok, counter := loop_check_that_candidates_have_question(f, f', question, ok, counter);
+      f', f'Empty, cands_have_question, exists_answer_true, exists_answer_false, counter := loop_check_that_candidates_have_question_and_that_it_isnt_trivial(f, f', question, exists_answer_true, exists_answer_false, counter);
+      assert cands_have_question ==> (exists_answer_true == (exists cand:candidate | cand in (f.Keys() - f'.Keys()) :: cand[question] == true));
+      assert cands_have_question ==> (exists_answer_false == (exists cand:candidate | cand in (f.Keys() - f'.Keys()) :: cand[question] == false));
     }
 
-    if ok {
+    var question_is_valid_and_not_trivial:bool := cands_have_question && exists_answer_true && exists_answer_false;
+
+    assert question_is_valid_and_not_trivial ==
+      ((forall cand:candidate | cand in f.Keys() :: question in cand.Keys) &&
+      (exists cand:candidate | cand in f.Keys() :: cand[question] == true) &&
+      (exists cand:candidate | cand in f.Keys() :: cand[question] == false));
+
+    if question_is_valid_and_not_trivial {
       var f_true:Map_Map_T<int, bool, bool>; f_true, counter := candidates_with_same_answer(f, question, true, counter);
       var f_false:Map_Map_T<int, bool, bool>; f_false, counter := candidates_with_same_answer(f, question, false, counter);
       var g_true:Map_Map_T<int, bool, int>; g_true, counter := candidates_with_same_answer(g, question, true, counter);
@@ -53,10 +67,93 @@ method verifyCDPC(f:Map_Map_T<int, bool, bool>, g:Map_Map_T<int, bool, int>, P:S
       var iv_true:Interview; iv_true, counter := iv.Get(true, counter);
       var iv_false:Interview; iv_false, counter := iv.Get(false, counter);
 
-      var b_true:bool; b_true, counter := verifyCDPC(f_true, g_true, P, a, b, x, y, iv_true, counter);
-      var b_false:bool; b_false, counter := verifyCDPC(f_false, g_false, P, a, b, x, y, iv_false, counter);
-      ok := ok && b_true && b_false;
+      var recursive_true:bool; recursive_true, counter := verifyCDPC(f_true, g_true, P, a, b, x, y, iv_true, counter);
+      var recursive_false:bool; recursive_false, counter := verifyCDPC(f_false, g_false, P, a, b, x, y, iv_false, counter);
+      var ok:bool := question_is_valid_and_not_trivial && recursive_true && recursive_false;
 
+      /*assert recursive_true == certificateCDPC(
+        (map c:candidate | c in f.Keys() && c[question] == true :: f.Model()[c]),
+        (map c:candidate | c in g.Keys() && c[question] == true :: g.Model()[c]),
+        P.Model(), a, b, x, y, iv.Model().True
+      );
+      assert recursive_false == certificateCDPC(
+        (map c:candidate | c in f.Keys() && c[question] == false :: f.Model()[c]),
+        (map c:candidate | c in g.Keys() && c[question] == false :: g.Model()[c]),
+        P.Model(), a, b, x, y, iv.Model().False
+      );*/
+
+
+
+      
+      // Problem preconditions
+      assert f.Valid() && g.Valid() && P.Valid() && iv.Valid();
+      assert forall c1, c2:candidate |  c1 in f.Keys() && c2 in f.Keys() :: c1.Keys == c2.Keys;
+      assert f.Keys() == g.Keys();
+      assert forall c:candidate | c in f.Keys() :: (P.Model() <= c.Keys);
+      assert 0.0 <= a <= b <= 1.0;
+      assert 0.0 <= x <= y <= 1.0;
+      // Information regarding the branch of the demonstration that we are focusing on
+      assert iv.Model() != Null;
+      assert question_is_valid_and_not_trivial == true;
+      // Variables that have been calculated
+      assert question == iv.Model().Key;
+      assume false;
+      assert question_is_valid_and_not_trivial ==
+        ((forall cand:candidate | cand in f.Keys() :: question in cand.Keys) &&
+        (exists cand:candidate | cand in f.Keys() :: cand[question] == true) &&
+        (exists cand:candidate | cand in f.Keys() :: cand[question] == false));
+      assert recursive_true ==
+        certificateCDPC(
+          (map c:candidate | c in f.Keys() && c[question] == true :: f.Model()[c]),
+          (map c:candidate | c in g.Keys() && c[question] == true :: g.Model()[c]),
+          P.Model(), a, b, x, y, iv.Model().True
+        );
+      assert recursive_false ==
+        certificateCDPC(
+          (map c:candidate | c in f.Keys() && c[question] == false :: f.Model()[c]),
+          (map c:candidate | c in g.Keys() && c[question] == false :: g.Model()[c]),
+          P.Model(), a, b, x, y, iv.Model().False
+        );
+      assert ok == question_is_valid_and_not_trivial && recursive_true && recursive_false;
+      assume false;
+      postcondition_verifyCDPC(f, g, P, a, b, x, y, iv, question, question_is_valid_and_not_trivial, recursive_true, recursive_false, ok);
+
+      /*
+      assume ok ==
+        ((forall cand:candidate | cand in f.Keys() :: question in cand.Keys) &&
+        (exists cand:candidate | cand in f.Keys() :: cand[question] == true) &&
+        (exists cand:candidate | cand in f.Keys() :: cand[question] == false))
+        &&
+        certificateCDPC(
+          (map c:candidate | c in f.Keys() && c[question] == true :: f.Model()[c]),
+          (map c:candidate | c in g.Keys() && c[question] == true :: g.Model()[c]),
+          P.Model(), a, b, x, y, iv.Model().True
+        )
+        &&
+        certificateCDPC(
+          (map c:candidate | c in f.Keys() && c[question] == false :: f.Model()[c]),
+          (map c:candidate | c in g.Keys() && c[question] == false :: g.Model()[c]),
+          P.Model(), a, b, x, y, iv.Model().False
+        );
+      assume ok ==
+        (forall cand:candidate | cand in f.Keys() :: question in cand.Keys) &&
+        (exists cand:candidate | cand in f.Keys() :: cand[question] == true) &&
+        (exists cand:candidate | cand in f.Keys() :: cand[question] == false)
+        &&
+        certificateCDPC(
+          (map c:candidate | c in f.Keys() && c[question] == true :: f.Model()[c]),
+          (map c:candidate | c in g.Keys() && c[question] == true :: g.Model()[c]),
+          P.Model(), a, b, x, y, iv.Model().True
+        )
+        &&
+        certificateCDPC(
+          (map c:candidate | c in f.Keys() && c[question] == false :: f.Model()[c]),
+          (map c:candidate | c in g.Keys() && c[question] == false :: g.Model()[c]),
+          P.Model(), a, b, x, y, iv.Model().False
+        );
+      assume r == certificateCDPC(f.Model(), g.Model(), P.Model(), a, b, x, y, iv.Model());
+      */
+      assume false;
       return ok, counter;
     }
 
@@ -66,25 +163,41 @@ method verifyCDPC(f:Map_Map_T<int, bool, bool>, g:Map_Map_T<int, bool, int>, P:S
 
 
 
-method loop_check_that_candidates_have_question(f:Map_Map_T<int, bool, bool>, f':Map_Map_T<int, bool, bool>, question:int, ok:bool, ghost counter_in:nat) returns (f'_out:Map_Map_T<int, bool, bool>, f'Empty:bool, ok_out:bool, ghost counter:nat)
-  requires in_universe_Map_Map_T(f', f)
-  requires ok == (forall cand:candidate | cand in (f.Keys() - f'.Keys()) :: question in cand.Keys)
-  requires 0 < f'.Cardinality()
-  ensures in_universe_Map_Map_T(f'_out, f)
-  ensures ok_out == (forall cand:candidate | cand in (f.Keys() - f'_out.Keys()) :: question in cand.Keys)
-  ensures f'_out.Cardinality() == f'.Cardinality() - 1
-  ensures f'Empty == (f'_out.Cardinality() == 0)
+method loop_check_that_candidates_have_question_and_that_it_isnt_trivial(f:Map_Map_T<int, bool, bool>, f'_in:Map_Map_T<int, bool, bool>, question:int, exists_answer_true:bool, exists_answer_false:bool, ghost counter_in:nat) returns (f':Map_Map_T<int, bool, bool>, f'_inEmpty:bool, cands_have_question:bool, exists_answer_true_out:bool, exists_answer_false_out:bool, ghost counter:nat)
+  requires in_universe_Map_Map_T(f'_in, f)
+  requires (forall cand:candidate | cand in (f.Keys() - f'_in.Keys()) :: question in cand.Keys)
+  requires exists_answer_true == (exists cand:candidate | cand in (f.Keys() - f'_in.Keys()) :: cand[question] == true)
+  requires exists_answer_false == (exists cand:candidate | cand in (f.Keys() - f'_in.Keys()) :: cand[question] == false)
+  requires 0 < f'_in.Cardinality()
+  ensures in_universe_Map_Map_T(f', f)
+  ensures cands_have_question == (forall cand:candidate | cand in (f.Keys() - f'.Keys()) :: question in cand.Keys)
+  ensures cands_have_question ==> (exists_answer_true_out == (exists cand:candidate | cand in (f.Keys() - f'.Keys()) :: cand[question] == true))
+  ensures cands_have_question ==> (exists_answer_false_out == (exists cand:candidate | cand in (f.Keys() - f'.Keys()) :: cand[question] == false))
+  ensures f'.Cardinality() == f'_in.Cardinality() - 1
+  ensures f'_inEmpty == (f'.Cardinality() == 0)
+  ensures counter <= counter_in + poly_loop_check_that_candidates_have_question_and_that_it_isnt_trivial(f)
 {
   counter := counter_in;
-  var cand:Map<int, bool>; cand, counter := f'.PickKey(counter);
-  f'_out, counter := f'.Remove(cand, counter);
+  in_universe_lemma_Map_Map_T(f'_in, f);
+  var cand:Map<int, bool>; cand, counter := f'_in.PickKey(counter);
+  assert counter <= counter_in + f.UBSize_Keys();
+  f', counter := f'_in.Remove(cand, counter);
   
-  var candHasQuestion:bool; candHasQuestion, counter := cand.ContainsKey(question, counter);
-  ok_out := ok && candHasQuestion;
+  cands_have_question, counter := cand.ContainsKey(question, counter);
+  
+  if cands_have_question {
+    var cand_answer:bool; cand_answer, counter := cand.Get(question, counter);
+    exists_answer_true_out := exists_answer_true || cand_answer;
+    exists_answer_false_out := exists_answer_false || !cand_answer;
+  }
+  else {
+    exists_answer_true_out := exists_answer_true;
+    exists_answer_false_out := exists_answer_false;
+  }
 
-  f'Empty, counter := f'_out.Empty(counter);
+  f'_inEmpty, counter := f'.Empty(counter);
 
-  return f'_out, f'Empty, ok_out, counter;
+  return f', f'_inEmpty, cands_have_question, exists_answer_true_out, exists_answer_false_out, counter;
 }
 
 
@@ -96,8 +209,8 @@ method correct_apt_ratio(f:Map_Map_T<int, bool, bool>, x:real, y:real, ghost cou
   requires f.Cardinality() != 0
   ensures var aptRatio:real := (|(set isApt:candidate | isApt in f.Keys() && f.Model()[isApt] :: isApt)| as real) / (f.Cardinality() as real);
           r == (aptRatio <= x || y <= aptRatio)
+  ensures counter <= counter_in + poly_correct_apt_ratio(f)
 {
-
   counter := counter_in;
   var f':Map_Map_T<int, bool, bool>; f', counter := f.Copy(counter);
   var f'Empty:bool; f'Empty, counter := f'.Empty(counter);
@@ -110,24 +223,9 @@ method correct_apt_ratio(f:Map_Map_T<int, bool, bool>, x:real, y:real, ghost cou
     invariant f'Empty == (f'.Cardinality() == 0)
     invariant numTotal == (f.Cardinality() - f'.Cardinality())
     invariant numApt == |(set aptCand:candidate | aptCand in (f.Keys() - f'.Keys()) && f.Model()[aptCand] :: aptCand)|
+    invariant counter <= counter_in + f.UBSize() + 1 + (f.Cardinality() - f'.Cardinality())*poly_correct_apt_ratio_loop(f)
   {
-    ghost var f'prev := f';
-    var cand:Map<int, bool>; cand, counter := f'.PickKey(counter);
-    f', counter := f'.Remove(cand, counter);
-    var isApt:bool; isApt, counter := f.Get(cand, counter);
-    if (isApt) {
-      numApt := numApt + 1;
-    }
-    assert numApt == |(set aptCand:candidate | aptCand in (f.Keys() - f'.Keys()) && f.Model()[aptCand] :: aptCand)| by {
-      assert f'prev.Keys() == (f'.Keys() + {cand.Model()});
-      assert (f.Keys() - (f'.Keys() + {cand.Model()})) == (f.Keys() - f'.Keys() - {cand.Model()});
-      assert if isApt then numApt == |(set aptCand:candidate | aptCand in (f.Keys() - f'.Keys() - {cand.Model()}) && f.Model()[aptCand] :: aptCand)| + 1
-            else           numApt == |(set aptCand:candidate | aptCand in (f.Keys() - f'.Keys() - {cand.Model()}) && f.Model()[aptCand] :: aptCand)|;
-      lemma_card_apt_set_when_remove_element(f.Model(), f.Keys() - f'.Keys(), cand.Model());
-    }
-
-    numTotal := numTotal + 1;
-    f'Empty, counter := f'.Empty(counter);
+    f', f'Empty, numApt, numTotal, counter := correct_apt_ratio_loop(f, f', numApt, numTotal, counter);
   }
   assert numTotal == f.Cardinality();
   identity_substraction_lemma(f.Keys(), f'.Keys());
@@ -137,6 +235,42 @@ method correct_apt_ratio(f:Map_Map_T<int, bool, bool>, x:real, y:real, ghost cou
   return (aptRatio <= x || y <= aptRatio), counter;
 }
 
+method correct_apt_ratio_loop(f:Map_Map_T<int, bool, bool>, f'_in:Map_Map_T<int, bool, bool>, numApt_in:int, numTotal_in:int, ghost counter_in:nat) returns (f':Map_Map_T<int, bool, bool>, f'Empty:bool, numApt:int, numTotal:int, ghost counter:nat)
+  requires in_universe_Map_Map_T(f'_in, f)
+  requires f'_in.Cardinality() != 0
+  requires numTotal_in == (f.Cardinality() - f'_in.Cardinality())
+  requires numApt_in == |(set aptCand:candidate | aptCand in (f.Keys() - f'_in.Keys()) && f.Model()[aptCand] :: aptCand)|
+
+  ensures f'.Cardinality() == f'_in.Cardinality() - 1
+  ensures in_universe_Map_Map_T(f', f)
+  ensures f'Empty == (f'.Cardinality() == 0)
+  ensures numTotal == (f.Cardinality() - f'.Cardinality())
+  ensures numApt == |(set aptCand:candidate | aptCand in (f.Keys() - f'.Keys()) && f.Model()[aptCand] :: aptCand)|
+  ensures counter <= counter_in + poly_correct_apt_ratio_loop(f)
+{
+  counter := counter_in;
+  in_universe_lemma_Map_Map_T(f'_in, f);
+  numApt := numApt_in;
+  numTotal := numTotal_in;
+  var cand:Map<int, bool>; cand, counter := f'_in.PickKey(counter);
+  assert counter <= counter_in + f.UBSize_Keys();
+  f', counter := f'_in.Remove(cand, counter);
+  var isApt:bool; isApt, counter := f.Get(cand, counter);
+  if (isApt) {
+    numApt := numApt + 1;
+  }
+  lemma_card_apt_set_when_remove_element(f.Model(), f.Keys() - f'.Keys(), cand.Model());
+  assert numApt == |(set aptCand:candidate | aptCand in (f.Keys() - f'.Keys()) && f.Model()[aptCand] :: aptCand)| by {
+    assert f'_in.Keys() == (f'.Keys() + {cand.Model()});
+    assert (f.Keys() - (f'.Keys() + {cand.Model()})) == (f.Keys() - f'.Keys() - {cand.Model()});
+    assert if isApt then numApt == |(set aptCand:candidate | aptCand in (f.Keys() - f'.Keys() - {cand.Model()}) && f.Model()[aptCand] :: aptCand)| + 1
+          else           numApt == |(set aptCand:candidate | aptCand in (f.Keys() - f'.Keys() - {cand.Model()}) && f.Model()[aptCand] :: aptCand)|;
+    lemma_card_apt_set_when_remove_element(f.Model(), f.Keys() - f'.Keys(), cand.Model());
+  }
+
+  numTotal := numTotal + 1;
+  f'Empty, counter := f'.Empty(counter);
+}
 
 
 method correct_private_ratio(f:Map_Map_T<int, bool, bool>, P:Set<int>, a:real, b:real, ghost counter_in:nat) returns (r:bool, ghost counter:nat)
@@ -151,12 +285,14 @@ method correct_private_ratio(f:Map_Map_T<int, bool, bool>, P:Set<int>, a:real, b
                   var privateRatio:real := (|(set isPrivate:candidate | isPrivate in f.Keys() && isPrivate[p] :: isPrivate)| as real) / (f.Cardinality() as real);
                   a <= privateRatio <= b
                 )
+  ensures counter <= counter_in + poly_correct_private_ratio(f, P)
 {
   counter := counter_in;
 
   r := true;
   var P':Set<int>; P', counter := P.Copy(counter);
   var P'Empty:bool; P'Empty, counter := P'.Empty(counter);
+  assert counter <= counter_in + P.UBSize0() + 1;
   while (!P'Empty)
     decreases P'.Cardinality()
     invariant in_universe_Set(P', P)
@@ -166,6 +302,7 @@ method correct_private_ratio(f:Map_Map_T<int, bool, bool>, P:Set<int>, a:real, b
                   var privateRatio:real := (|(set isPrivate:candidate | isPrivate in f.Keys() && isPrivate[p] :: isPrivate)| as real) / (f.Cardinality() as real);
                   a <= privateRatio <= b
                 )
+    invariant counter <= counter_in + P.UBSize0() + 1 + (P.Cardinality() - P'.Cardinality())*poly_correct_private_ratio_outer_loop(f, P)
   {
     r, P', P'Empty, counter := correct_private_ratio_outer_loop(f, P, P', a, b, r, counter);
   }
@@ -175,35 +312,37 @@ method correct_private_ratio(f:Map_Map_T<int, bool, bool>, P:Set<int>, a:real, b
 }
 
 
-method correct_private_ratio_outer_loop(f:Map_Map_T<int, bool, bool>, P:Set<int>, P':Set<int>, a:real, b:real, r:bool, ghost counter_in:nat) returns (r_out:bool, P'_out:Set<int>, P'Empty:bool, ghost counter:nat)
+method correct_private_ratio_outer_loop(f:Map_Map_T<int, bool, bool>, P:Set<int>, P'_in:Set<int>, a:real, b:real, r_in:bool, ghost counter_in:nat) returns (r:bool, P':Set<int>, P'Empty:bool, ghost counter:nat)
   requires f.Valid()
   requires forall c1, c2:candidate |  c1 in f.Keys() && c2 in f.Keys() :: c1.Keys == c2.Keys
   requires 0.0 <= a <= b <= 1.0
   requires forall c:candidate | c in f.Keys() :: (P.Model() <= c.Keys)
   requires f.Cardinality() != 0
 
-  requires in_universe_Set(P', P)
-  requires P'.Cardinality() != 0
-  requires r == forall p:int | p in (P.Model() - P'.Model()) ::
+  requires in_universe_Set(P'_in, P)
+  requires P'_in.Cardinality() != 0
+  requires r_in == forall p:int | p in (P.Model() - P'_in.Model()) ::
               (
                 var privateRatio:real := (|(set isPrivate:candidate | isPrivate in f.Keys() && isPrivate[p] :: isPrivate)| as real) / (f.Cardinality() as real);
                 a <= privateRatio <= b
               )
   
-  ensures P'_out.Cardinality() < P'.Cardinality()
-  ensures in_universe_Set(P'_out, P)
-  ensures P'Empty == (P'_out.Cardinality() == 0)
-  ensures r_out == forall p:int | p in (P.Model() - P'_out.Model()) ::
+  ensures P'.Cardinality() == P'_in.Cardinality() - 1
+  ensures in_universe_Set(P', P)
+  ensures P'Empty == (P'.Cardinality() == 0)
+  ensures r == forall p:int | p in (P.Model() - P'.Model()) ::
               (
                 var privateRatio:real := (|(set isPrivate:candidate | isPrivate in f.Keys() && isPrivate[p] :: isPrivate)| as real) / (f.Cardinality() as real);
                 a <= privateRatio <= b
               )
-
+  ensures counter <= counter_in + poly_correct_private_ratio_outer_loop(f, P)
 {
   counter := counter_in;
-  var p:int; p, counter := P'.Pick(counter);
+  var p:int; p, counter := P'_in.Pick(counter);
   
-  P'_out, counter := P'.Remove(p, counter);
+  P', counter := P'_in.Remove(p, counter);
+  in_universe_lemma_Set(P'_in, P);
+  in_universe_lemma_Set(P', P);
 
   var f':Map_Map_T<int, bool, bool>; f', counter := f.Copy(counter);
   var numPriv:int := 0;
@@ -216,66 +355,73 @@ method correct_private_ratio_outer_loop(f:Map_Map_T<int, bool, bool>, P:Set<int>
     invariant numTotal == (f.Cardinality() - f'.Cardinality())
     invariant numPriv == |(set privCand:candidate | privCand in (f.Keys() - f'.Keys()) && privCand[p] :: privCand)|
     invariant f'Empty == (f'.Cardinality() == 0)
+    invariant counter <= counter_in + f.UBSize() + P.UBSize0() + 2 + (f.Cardinality() - f'.Cardinality())*poly_correct_private_ratio_inner_loop(f)
   {
+    //ghost var f'_prev := f';
     f', f'Empty, numTotal, numPriv, counter := correct_private_ratio_inner_loop(f, f', p, numTotal, numPriv, counter);
+    //correct_private_ratio_outer_loop_restore_counter_invariant(f, f', f'_prev, P, counter, counter_in);
+    //restore_counter_invariant(f.Cardinality(), f'.Cardinality(), f'_prev.Cardinality(), f.UBSize() + P.UBSize0() + 2, poly_correct_private_ratio_inner_loop(f), counter, counter_in);
   }
   identity_substraction_lemma(f.Keys(), f'.Keys());
   var privateRatio:real := (numPriv as real) / (numTotal as real);
 
-  r_out := r && (a <= privateRatio <= b);
-  P'Empty, counter := P'_out.Empty(counter);
+  r := r_in && (a <= privateRatio <= b);
+  P'Empty, counter := P'.Empty(counter);
 
 
   assert privateRatio == (|(set isPrivate:candidate | isPrivate in f.Keys() && isPrivate[p] :: isPrivate)| as real) / (f.Cardinality() as real) by {
     assert (numTotal as real) == (f.Cardinality() as real);
     assert (numPriv as real) == (|(set isPrivate:candidate | isPrivate in f.Keys() && isPrivate[p] :: isPrivate)| as real);
   }
-  lemma_private_ratio(f, P, P', P'_out, a, b, r, r_out, p, privateRatio);
+  lemma_private_ratio(f, P, P'_in, P', a, b, r_in, r, p, privateRatio);
   
-  return r_out, P'_out, P'Empty, counter;
+  return r, P', P'Empty, counter;
 }
 
 
-method correct_private_ratio_inner_loop(f:Map_Map_T<int, bool, bool>, f':Map_Map_T<int, bool, bool>, p:int, numTotal:int, numPriv:int, ghost counter_in:nat) returns (f'_out:Map_Map_T<int, bool, bool>, f'_Empty:bool, numTotal':int, numPriv':int, ghost counter:nat)
+method correct_private_ratio_inner_loop(f:Map_Map_T<int, bool, bool>, f'_in:Map_Map_T<int, bool, bool>, p:int, numTotal_in:int, numPriv_in:int, ghost counter_in:nat) returns (f':Map_Map_T<int, bool, bool>, f'Empty:bool, numTotal:int, numPriv:int, ghost counter:nat)
   requires f.Valid()
   requires forall c1, c2:candidate |  c1 in f.Keys() && c2 in f.Keys() :: c1.Keys == c2.Keys
   requires forall c:candidate | c in f.Keys() :: (p in c.Keys)
   requires f.Cardinality() != 0
-  requires f'.Cardinality() != 0
+  requires f'_in.Cardinality() != 0
   
-  requires in_universe_Map_Map_T(f', f)
-  requires numTotal == (f.Cardinality() - f'.Cardinality())
-  requires numPriv == |(set privCand:candidate | privCand in (f.Keys() - f'.Keys()) && privCand[p] :: privCand)|
+  requires in_universe_Map_Map_T(f'_in, f)
+  requires numTotal_in == (f.Cardinality() - f'_in.Cardinality())
+  requires numPriv_in == |(set privCand:candidate | privCand in (f.Keys() - f'_in.Keys()) && privCand[p] :: privCand)|
   
-  ensures f'_out.Cardinality() < f'.Cardinality()
+  ensures f'.Cardinality() == f'_in.Cardinality() - 1
   
-  ensures in_universe_Map_Map_T(f'_out, f)
-  ensures numTotal' == (f.Cardinality() - f'_out.Cardinality())
-  ensures numPriv' == |(set privCand:candidate | privCand in (f.Keys() - f'_out.Keys()) && privCand[p] :: privCand)|
-  ensures f'_Empty == (f'_out.Cardinality() == 0)
+  ensures in_universe_Map_Map_T(f', f)
+  ensures numTotal == (f.Cardinality() - f'.Cardinality())
+  ensures numPriv == |(set privCand:candidate | privCand in (f.Keys() - f'.Keys()) && privCand[p] :: privCand)|
+  ensures f'Empty == (f'.Cardinality() == 0)
+  ensures counter <= counter_in + poly_correct_private_ratio_inner_loop(f)
 {
   counter := counter_in;
-  numPriv' := numPriv;
+  numPriv := numPriv_in;
 
-  var cand:Map<int, bool>; cand, counter := f'.PickKey(counter);
-  f'_out, counter := f'.Remove(cand, counter);
+  var cand:Map<int, bool>; cand, counter := f'_in.PickKey(counter);
+  f', counter := f'_in.Remove(cand, counter);
+  in_universe_lemma_Map_Map_T(f'_in, f);
+  in_universe_lemma_Map_Map_T(f', f);
   var isPrivate:bool; isPrivate, counter := cand.Get(p, counter);
   if (isPrivate) {
-    numPriv' := numPriv + 1;
+    numPriv := numPriv_in + 1;
   }
 
-  assert numPriv' == |(set privCand:candidate | privCand in (f.Keys() - f'_out.Keys()) && privCand[p] :: privCand)| by {
-    assert f'.Keys() == (f'_out.Keys() + {cand.Model()});
-    assert (f.Keys() - (f'_out.Keys() + {cand.Model()})) == (f.Keys() -f'_out.Keys() - {cand.Model()});
-    assert if isPrivate then numPriv' == |(set privCand:candidate | privCand in (f.Keys() - f'_out.Keys() - {cand.Model()}) && privCand[p] :: privCand)| + 1
-            else           numPriv' == |(set privCand:candidate | privCand in (f.Keys() - f'_out.Keys() - {cand.Model()}) && privCand[p] :: privCand)|;
-    lemma_card_priv_set_when_remove_element(f.Model(), f.Keys() - f'_out.Keys(), cand.Model(), p);
+  assert numPriv == |(set privCand:candidate | privCand in (f.Keys() - f'.Keys()) && privCand[p] :: privCand)| by {
+    assert f'_in.Keys() == (f'.Keys() + {cand.Model()});
+    assert (f.Keys() - (f'.Keys() + {cand.Model()})) == (f.Keys() -f'.Keys() - {cand.Model()});
+    assert if isPrivate then numPriv == |(set privCand:candidate | privCand in (f.Keys() - f'.Keys() - {cand.Model()}) && privCand[p] :: privCand)| + 1
+            else           numPriv == |(set privCand:candidate | privCand in (f.Keys() - f'.Keys() - {cand.Model()}) && privCand[p] :: privCand)|;
+    lemma_card_priv_set_when_remove_element(f.Model(), f.Keys() - f'.Keys(), cand.Model(), p);
   }
   
-  numTotal' := numTotal + 1;
-  f'_Empty, counter := f'_out.Empty(counter);
+  numTotal := numTotal_in + 1;
+  f'Empty, counter := f'.Empty(counter);
 
-  return f'_out, f'_Empty, numTotal', numPriv', counter;
+  return f', f'Empty, numTotal, numPriv, counter;
 }
 
 
@@ -286,7 +432,7 @@ method candidates_with_same_answer<T>(f:Map_Map_T<int, bool, T>, question:int, a
   requires forall c:candidate |  c in f.Keys() :: question in c
   ensures f_out.Valid()
   ensures f_out.Model() == (map c:candidate | c in f.Keys() && c[question] == answer :: f.Model()[c])
-  //ensures counter <= counter_in + poly_candidates_with_same_answer(f)
+  ensures counter <= counter_in + poly_candidates_with_same_answer(f)
 {
   counter := counter_in;
 
@@ -311,73 +457,125 @@ method candidates_with_same_answer<T>(f:Map_Map_T<int, bool, T>, question:int, a
     invariant f'Empty == (f'.Cardinality() == 0)
   {
     ghost var f'_prev := f';
-    assert counter <= counter_in + f.UBSize() + 2 + (f.Cardinality() - f'.Cardinality())*poly_candidates_with_same_answer_loop(f);
     f', f_out, f'Empty, counter := candidates_with_same_answer_loop(f, f', f_out, question, answer, counter);
-    
-    assert counter <= counter_in + f.UBSize() + 2 + (f.Cardinality() - f'.Cardinality())*poly_candidates_with_same_answer_loop(f) by {
-      assert counter <= counter_in + f.UBSize() + 2 + (f.Cardinality() - f'_prev.Cardinality())*poly_candidates_with_same_answer_loop(f) + poly_candidates_with_same_answer_loop(f);
-      assert f'_prev.Cardinality() == (f'.Cardinality() + 1);
-      assert (f.Cardinality() - f'_prev.Cardinality()) == (f.Cardinality() - (f'.Cardinality() + 1));
-      assume (f.Cardinality() - f'_prev.Cardinality())*poly_candidates_with_same_answer_loop(f) == (f.Cardinality() - (f'.Cardinality() + 1))*poly_candidates_with_same_answer_loop(f);
-      assert counter <= counter_in + f.UBSize() + 2 + (f.Cardinality() - (f'.Cardinality() + 1))*poly_candidates_with_same_answer_loop(f) + poly_candidates_with_same_answer_loop(f);
-    }
+    candidates_with_same_answer_restore_counter_invariant(f, f', f'_prev, counter, counter_in);
   }
-  identity_substraction_lemma(f.Keys(), f'.Keys());
+  candidates_with_same_answer_counter_simplification(f, f', counter, counter_in);
+  assert counter <= counter_in + poly_candidates_with_same_answer(f);
 
   return f_out, counter;
 }
 
 
-method candidates_with_same_answer_loop<T>(f:Map_Map_T<int, bool, T>, f':Map_Map_T<int, bool, T>, f'':Map_Map_T<int, bool, T>, question:int, answer:bool, ghost counter_in:nat) returns (f'_out:Map_Map_T<int, bool, T>, f''_out:Map_Map_T<int, bool, T>, f'Empty:bool, ghost counter:nat)
+method candidates_with_same_answer_loop<T>(f:Map_Map_T<int, bool, T>, f'_in:Map_Map_T<int, bool, T>, f''_in:Map_Map_T<int, bool, T>, question:int, answer:bool, ghost counter_in:nat) returns (f':Map_Map_T<int, bool, T>, f'':Map_Map_T<int, bool, T>, f'Empty:bool, ghost counter:nat)
   requires forall c1, c2:candidate |  c1 in f.Keys() && c2 in f.Keys() :: c1.Keys == c2.Keys
   requires forall c:candidate |  c in f.Keys() :: question in c
 
-  requires in_universe_Map_Map_T(f', f)
-  requires in_universe_Map_Map_T(f'', f)
-  requires f'.Cardinality() != 0
-  requires f''.Model() == (map c:candidate | c in (f.Keys() - f'.Keys()) && c[question] == answer :: f.Model()[c])
+  requires in_universe_Map_Map_T(f'_in, f)
+  requires in_universe_Map_Map_T(f''_in, f)
+  requires f'_in.Cardinality() != 0
+  requires f''_in.Model() == (map c:candidate | c in (f.Keys() - f'_in.Keys()) && c[question] == answer :: f.Model()[c])
 
-  ensures f'_out.Cardinality() == f'.Cardinality() - 1
+  ensures f'.Cardinality() == f'_in.Cardinality() - 1
 
-  ensures in_universe_Map_Map_T(f'_out, f)
-  ensures in_universe_Map_Map_T(f''_out, f)
-  ensures f'Empty == (f'_out.Cardinality() == 0)
+  ensures in_universe_Map_Map_T(f', f)
+  ensures in_universe_Map_Map_T(f'', f)
+  ensures f'Empty == (f'.Cardinality() == 0)
   
-  ensures f''_out.Model() == (map c:candidate | c in (f.Keys() - f'_out.Keys()) && c[question] == answer :: f.Model()[c])
+  ensures f''.Model() == (map c:candidate | c in (f.Keys() - f'.Keys()) && c[question] == answer :: f.Model()[c])
   ensures counter <= counter_in + poly_candidates_with_same_answer_loop(f)
 {
-  in_universe_lemma_Map_Map_T(f', f);
-  in_universe_lemma_Map_Map_T(f'', f);
+  in_universe_lemma_Map_Map_T(f'_in, f);
+  in_universe_lemma_Map_Map_T(f''_in, f);
 
   counter := counter_in;
-  var cand:Map<int, bool>; cand, counter := f'.PickKey(counter);
-  f'_out, counter := f'.Remove(cand, counter);
+  var cand:Map<int, bool>; cand, counter := f'_in.PickKey(counter);
+  f', counter := f'_in.Remove(cand, counter);
 
   var cand_answer:bool; cand_answer, counter := cand.Get(question, counter);
 
   if (cand_answer == answer) {
     var f_cand:T; f_cand, counter := f.Get(cand, counter);
-    f''_out, counter := f''.Insert(cand, f_cand, counter);
+    f'', counter := f''_in.Insert(cand, f_cand, counter);
 
-    assert (forall k | k in f''.Universe().Keys :: f''_out.Universe()[k] == f.Universe()[k]);
-    candidates_with_same_answer_lemma_1<T>(f, f',  f'', f'_out, f''_out, cand, question, answer);
+    assert (forall k | k in f''_in.Universe().Keys :: f''.Universe()[k] == f.Universe()[k]);
+    candidates_with_same_answer_lemma_1<T>(f, f'_in, f''_in, f', f'', cand, question, answer);
     //assert counter <= counter_in + 3*f.UBSize() + 2*f.UBSize_Keys();
   }
   else {
-    f''_out, counter := f''.Copy(counter);
-    candidates_with_same_answer_lemma_2(f, f',  f'', f'_out, f''_out, cand, question, answer);
+    f'', counter := f''_in.Copy(counter);
+    candidates_with_same_answer_lemma_2(f, f'_in,  f''_in, f', f'', cand, question, answer);
     //assert counter <= counter_in + 2*f.UBSize() + 2*f.UBSize_Keys();
   }
 
-  f'Empty, counter := f'_out.Empty(counter);
+  f'Empty, counter := f'.Empty(counter);
 
-  reveal poly_candidates_with_same_answer_loop(f);    // ?
-  return f'_out, f''_out, f'Empty, counter;
+  return f', f'', f'Empty, counter;
 }
+
+
+
 
 
 // POLYNOMIALS
 
+
+
+
+
+ghost function poly_loop_check_that_candidates_have_question_and_that_it_isnt_trivial<T>(f:Map_Map_T<int, bool, T>) : (o:nat)
+{
+  f.UBSize() + 3*f.UBSize_Keys() + 1
+}
+
+ghost function poly_correct_apt_ratio<T>(f:Map_Map_T<int, bool, T>) : (o:nat)
+  ensures f.UBSize() + 1 + f.Cardinality()*poly_correct_apt_ratio_loop(f) <= o
+{
+  /*calc == {
+    f.UBSize() + 1 + f.Cardinality()*poly_correct_apt_ratio_loop(f);
+    f.UBSize() + 1 + f.Cardinality()*(2*f.UBSize() + f.UBSize_Keys() + 1);
+    f.UBSize() + 1 + (2*f.UBSize()*f.Cardinality() + f.UBSize_Keys()*f.Cardinality() + f.Cardinality());
+    f.UBSize() + 1 + (2*f.UBSize()*f.Cardinality() + f.UBSize() + f.Cardinality());
+    2*f.UBSize()*f.Cardinality() + 2*f.UBSize() + f.Cardinality() + 1;
+  }*/
+  2*f.UBSize()*f.Cardinality() + 2*f.UBSize() + f.Cardinality() + 1
+}
+
+ghost function poly_correct_apt_ratio_loop<T>(f:Map_Map_T<int, bool, T>) : (o:nat)
+{
+  2*f.UBSize() + f.UBSize_Keys() + 1
+}
+
+ghost function poly_correct_private_ratio<T>(f:Map_Map_T<int, bool, T>, P:Set<int>) : (o:nat)
+  ensures P.UBSize0() + 1 + P.Cardinality()*poly_correct_private_ratio_outer_loop(f, P) <= o
+{
+  /*calc == {
+    P.UBSize0() + 1 + P.Cardinality()*poly_correct_private_ratio_outer_loop(f, P);
+    P.UBSize0() + 1 + P.Cardinality()*(f.UBSize()*f.Cardinality() + 3*f.UBSize() + f.Cardinality() + P.UBSize0() + 3);
+    P.UBSize0() + 1 + (f.UBSize()*f.Cardinality()*P.Cardinality() + 3*f.UBSize()*P.Cardinality() + f.Cardinality()*P.Cardinality() + P.UBSize0()*P.Cardinality() + 3*P.Cardinality());
+    f.UBSize()*f.Cardinality()*P.Cardinality() + 3*f.UBSize()*P.Cardinality() + f.Cardinality()*P.Cardinality() + P.UBSize0()*P.Cardinality() + 3*P.Cardinality() + P.UBSize0() + 1;
+  }*/
+  f.UBSize()*f.Cardinality()*P.Cardinality() + 3*f.UBSize()*P.Cardinality() + f.Cardinality()*P.Cardinality() + P.UBSize0()*P.Cardinality() + 3*P.Cardinality() + P.UBSize0() + 1
+}
+
+ghost function poly_correct_private_ratio_outer_loop<T>(f:Map_Map_T<int, bool, T>, P:Set<int>) : (o:nat)
+  ensures f.UBSize() + P.UBSize0() + 3 + f.Cardinality()*poly_correct_private_ratio_inner_loop(f) <= o
+{
+  /*calc == {
+    f.UBSize() + P.UBSize0() + 3 + f.Cardinality()*poly_correct_private_ratio_inner_loop(f);
+    f.UBSize() + P.UBSize0() + 3 + f.Cardinality()*(f.UBSize() + 2*f.UBSize_Keys() + 1);
+    f.UBSize() + P.UBSize0() + 3 + (f.UBSize()*f.Cardinality() + 2*f.UBSize_Keys()*f.Cardinality() + f.Cardinality());
+    f.UBSize() + f.UBSize()*f.Cardinality() + 2*f.UBSize_Keys()*f.Cardinality() + f.Cardinality() + P.UBSize0() + 3;
+    f.UBSize() + f.UBSize()*f.Cardinality() + 2*f.UBSize() + f.Cardinality() + P.UBSize0() + 3;
+    f.UBSize()*f.Cardinality() + 3*f.UBSize() + f.Cardinality() + P.UBSize0() + 3;
+  }*/
+  f.UBSize()*f.Cardinality() + 3*f.UBSize() + f.Cardinality() + P.UBSize0() + 3
+}
+
+ghost function poly_correct_private_ratio_inner_loop<T>(f:Map_Map_T<int, bool, T>) : (o:nat)
+{
+  f.UBSize() + 2*f.UBSize_Keys() + 1
+}
 
 ghost function poly_candidates_with_same_answer<T>(f:Map_Map_T<int, bool, T>) : (o:nat)
 {
@@ -390,12 +588,18 @@ ghost function poly_candidates_with_same_answer<T>(f:Map_Map_T<int, bool, T>) : 
   3*f.UBSize()*f.Cardinality() + 2*f.UBSize_Keys()*f.Cardinality() + f.UBSize() + f.Cardinality() + 2
 }
 
-ghost opaque function poly_candidates_with_same_answer_loop<T>(f:Map_Map_T<int, bool, T>) : (o:nat)
+ghost function poly_candidates_with_same_answer_loop<T>(f:Map_Map_T<int, bool, T>) : (o:nat)
 {
   3*f.UBSize() + 2*f.UBSize_Keys() + 1
 }
 
+
+
+
+
 // LEMMAS
+
+
 
 
 
@@ -567,3 +771,115 @@ lemma candidates_with_same_answer_lemma_2_aux<T>(f:Map_Map_T<int, bool, T>, f'_o
   ensures (map c:candidate | c in (f.Keys() - f'_out.Keys() - {cand.Model()}) && c[question] == answer :: f.Model()[c]) ==
           (map c:candidate | c in (f.Keys() - f'_out.Keys()) && c[question] == answer :: f.Model()[c])
 {}
+
+lemma candidates_with_same_answer_restore_counter_invariant<T>(f:Map_Map_T<int, bool, T>, f':Map_Map_T<int, bool, T>, f'_prev:Map_Map_T<int, bool, T>, counter:nat, counter_in:nat)
+requires counter <= counter_in + f.UBSize() + 2 + (f.Cardinality() - f'_prev.Cardinality())*poly_candidates_with_same_answer_loop(f) + poly_candidates_with_same_answer_loop(f)
+requires f'_prev.Cardinality() == (f'.Cardinality() + 1)
+ensures counter <= counter_in + f.UBSize() + 2 + (f.Cardinality() - f'.Cardinality())*poly_candidates_with_same_answer_loop(f)
+{
+  /*assert (f.Cardinality() - f'_prev.Cardinality()) == (f.Cardinality() - (f'.Cardinality() + 1));
+  assert (f.Cardinality() - f'_prev.Cardinality())*poly_candidates_with_same_answer_loop(f) == (f.Cardinality() - (f'.Cardinality() + 1))*poly_candidates_with_same_answer_loop(f);
+  assert counter <= counter_in + f.UBSize() + 2 + (f.Cardinality() - (f'.Cardinality() + 1))*poly_candidates_with_same_answer_loop(f) + poly_candidates_with_same_answer_loop(f);*/
+}
+
+/*lemma correct_private_ratio_outer_loop_restore_counter_invariant<T>(f:Map_Map_T<int, bool, T>, f':Map_Map_T<int, bool, T>, f'_prev:Map_Map_T<int, bool, T>, P:Set<int>, counter:nat, counter_in:nat)
+requires counter <= counter_in + f.UBSize() + P.UBSize0() + 2 + (f.Cardinality() - f'_prev.Cardinality())*poly_correct_private_ratio_inner_loop(f) + poly_correct_private_ratio_inner_loop(f)
+requires f'_prev.Cardinality() == (f'.Cardinality() + 1)
+ensures counter <= counter_in + f.UBSize() + P.UBSize0() + 2 + (f.Cardinality() - f'.Cardinality())*poly_correct_private_ratio_inner_loop(f)
+{
+}
+
+lemma restore_counter_invariant(card:nat, card':nat, card'_prev:nat, counter_before:nat, counter_loop:nat, counter:nat, counter_in:nat)
+requires counter <= counter_in + counter_before + (card - card'_prev)*counter_loop + counter_loop
+requires card'_prev == (card' + 1)
+ensures counter <= counter_in + counter_before + (card - card')*counter_loop
+{
+}*/
+
+lemma candidates_with_same_answer_counter_simplification<T>(f:Map_Map_T<int, bool, T>, f':Map_Map_T<int, bool, T>, counter:nat, counter_in:nat)
+  requires f'.Cardinality() == 0
+  requires counter <= counter_in + f.UBSize() + 2 + (f.Cardinality() - f'.Cardinality())*poly_candidates_with_same_answer_loop(f)
+  ensures counter <= counter_in + poly_candidates_with_same_answer(f)
+{
+  //identity_substraction_lemma(f.Keys(), f'.Keys());
+  //assert counter <= counter_in + f.UBSize() + 2 + f.Cardinality()*poly_candidates_with_same_answer_loop(f);
+}
+
+lemma postcondition_verifyCDPC(f:Map_Map_T<int, bool, bool>, g:Map_Map_T<int, bool, int>, P:Set<int>, a:real, b:real, x:real, y:real, iv:Interview, question:int, question_is_valid_and_not_trivial:bool, recursive_true:bool, recursive_false:bool, ok:bool)
+  // Problem preconditions
+  requires f.Valid() && g.Valid() && P.Valid() && iv.Valid()
+  requires forall c1, c2:candidate |  c1 in f.Keys() && c2 in f.Keys() :: c1.Keys == c2.Keys
+  requires f.Keys() == g.Keys()
+  requires forall c:candidate | c in f.Keys() :: (P.Model() <= c.Keys)
+  requires 0.0 <= a <= b <= 1.0
+  requires 0.0 <= x <= y <= 1.0
+  // Information regarding the branch of the demonstration that we are focusing on
+  requires iv.Model() != Null
+  requires question_is_valid_and_not_trivial == true
+  // Variables that have been calculated
+  requires question == iv.Model().Key
+  requires question_is_valid_and_not_trivial ==
+    ((forall cand:candidate | cand in f.Keys() :: question in cand.Keys) &&
+    (exists cand:candidate | cand in f.Keys() :: cand[question] == true) &&
+    (exists cand:candidate | cand in f.Keys() :: cand[question] == false))
+  requires recursive_true ==
+    certificateCDPC(
+      (map c:candidate | c in f.Keys() && c[question] == true :: f.Model()[c]),
+      (map c:candidate | c in g.Keys() && c[question] == true :: g.Model()[c]),
+      P.Model(), a, b, x, y, iv.Model().True
+    )
+  requires recursive_false ==
+    certificateCDPC(
+      (map c:candidate | c in f.Keys() && c[question] == false :: f.Model()[c]),
+      (map c:candidate | c in g.Keys() && c[question] == false :: g.Model()[c]),
+      P.Model(), a, b, x, y, iv.Model().False
+    )
+  requires ok == question_is_valid_and_not_trivial && recursive_true && recursive_false
+  // Postcondition
+  ensures ok == certificateCDPC(f.Model(), g.Model(), P.Model(), a, b, x, y, iv.Model())
+{}
+
+
+ghost predicate pred_problem_preconditions(f:Map_Map_T<int, bool, bool>, g:Map_Map_T<int, bool, int>, P:Set<int>, a:real, b:real, x:real, y:real, iv:Interview)
+{
+  (f.Valid() && g.Valid() && P.Valid() && iv.Valid()) &&
+  (forall c1, c2:candidate |  c1 in f.Keys() && c2 in f.Keys() :: c1.Keys == c2.Keys) &&
+  (f.Keys() == g.Keys()) &&
+  (forall c:candidate | c in f.Keys() :: (P.Model() <= c.Keys)) &&
+  (0.0 <= a <= b <= 1.0) &&
+  (0.0 <= x <= y <= 1.0)
+}
+
+ghost predicate pred_branch_info(iv:Interview, question_is_valid_and_not_trivial:bool)
+{
+  (iv.Model() != Null) &&
+  (question_is_valid_and_not_trivial == true)
+}
+
+ghost predicate pred_calc_variables(f:Map_Map_T<int, bool, bool>, g:Map_Map_T<int, bool, int>, P:Set<int>, a:real, b:real, x:real, y:real, iv:Interview, question:int, question_is_valid_and_not_trivial:bool, recursive_true:bool, recursive_false:bool, ok:bool)
+  requires pred_problem_preconditions(f, g, P, a, b, x, y, iv) && pred_branch_info(iv, question_is_valid_and_not_trivial)
+{
+  (question == iv.Model().Key) &&
+  (question_is_valid_and_not_trivial ==
+    ((forall cand:candidate | cand in f.Keys() :: question in cand.Keys) &&
+    (exists cand:candidate | cand in f.Keys() :: cand[question] == true) &&
+    (exists cand:candidate | cand in f.Keys() :: cand[question] == false))
+  ) &&
+  (recursive_true ==
+    certificateCDPC(
+      (map c:candidate | c in f.Keys() && c[question] == true :: f.Model()[c]),
+      (map c:candidate | c in g.Keys() && c[question] == true :: g.Model()[c]),
+      P.Model(), a, b, x, y, iv.Model().True
+    )
+  ) &&
+  (recursive_false ==
+    certificateCDPC(
+      (map c:candidate | c in f.Keys() && c[question] == false :: f.Model()[c]),
+      (map c:candidate | c in g.Keys() && c[question] == false :: g.Model()[c]),
+      P.Model(), a, b, x, y, iv.Model().False
+    )
+  ) &&
+  (ok == question_is_valid_and_not_trivial && recursive_true && recursive_false)
+}
+
+
